backend/Unusedglobproof.v
@@ -847,62 +847,19 @@ Inductive match_states: state -> state -> Prop :=
          (MEMINJ: Mem.inject j (flat_frameinj (length (Mem.stack_adt m))) m tm),
       match_states (State s f (Vptr sp Ptrofs.zero) pc rs m)
                    (State ts f (Vptr tsp Ptrofs.zero) pc trs tm)
-  | match_states_call: forall s fd args m ts targs tm j sz tc
+  | match_states_call: forall s fd args m ts targs tm j sz
          (STACKS: match_stacks j s ts (Mem.nextblock m) (Mem.nextblock tm))
          (KEPT: forall id, ref_fundef fd id -> kept id)
          (ARGINJ: Val.inject_list j args targs)
-         (MEMINJ: Mem.inject j (flat_frameinj (length (Mem.stack_adt m))) m tm)
-         (TAILNOPERM: tc = true -> Mem.top_tframe_no_perm (Mem.perm tm) (Mem.stack_adt tm)),
-      match_states (Callstate s fd args m sz tc)
-                   (Callstate ts fd targs tm sz tc)
+         (MEMINJ: Mem.inject j (flat_frameinj (length (Mem.stack_adt m))) m tm),
+      match_states (Callstate s fd args m sz)
+                   (Callstate ts fd targs tm sz)
   | match_states_return: forall s res m ts tres tm j 
          (STACKS: match_stacks j s ts (Mem.nextblock m) (Mem.nextblock tm))
          (RESINJ: Val.inject j res tres)
          (MEMINJ: Mem.inject j (flat_frameinj (length (Mem.stack_adt m))) m tm),
       match_states (Returnstate s res m)
                    (Returnstate ts tres tm).
-
-Lemma stack_equiv_inv_step:
-  forall S1 t S2
-    (STEP: step fn_stack_requirements ge S1 t S2)
-    S1' (MS: match_states S1 S1')
-    S2' (STEP': step fn_stack_requirements tge S1' t S2')
-    (SEI: stack_equiv_inv S1 S1'),
-    stack_equiv_inv S2 S2'.
-Proof.
-  intros.
-  inv STEP; inv MS; inv STEP'; try congruence;
-    unfold stack_equiv_inv in *; simpl in *; repeat rewrite_stack_blocks; eauto.
-  - revert EQ EQ0. repeat rewrite_stack_blocks. intros A B; rewrite A, B. simpl.
-    inv SEI. constructor. simpl; auto.
-  - revert SEI. rewrite <- (Mem.alloc_stack_blocks _ _ _ _ _ H).
-    rewrite <- (Mem.alloc_stack_blocks _ _ _ _ _ H8).
-    intro STRUCT.
-    destruct tc.
-    rewrite EQ1, EQ0 in STRUCT. inv STRUCT; constructor; auto.
-    constructor; auto.
-    rewrite Mem.push_new_stage_stack in EQ1, EQ0. inv EQ1; inv EQ0. constructor; auto.
-    constructor; auto. constructor.
-Qed.
-
-Lemma external_call_inject:
-  forall ef vargs m1 t vres m2 f g m1' vargs',
-  meminj_preserves_globals f ->
-  external_call ef ge vargs m1 t vres m2 ->
-  Mem.inject f g m1 m1' ->
-  Val.inject_list f vargs vargs' ->
-  exists f', exists vres', exists m2',
-    external_call ef tge vargs' m1' t vres' m2'
-    /\ Val.inject f' vres vres'
-    /\ Mem.inject f' g m2 m2'
-    /\ Mem.unchanged_on (loc_unmapped f) m1 m2
-    /\ Mem.unchanged_on (loc_out_of_reach f m1) m1' m2'
-    /\ inject_incr f f'
-    /\ inject_separated f f' m1 m1'.
-Proof.
-  intros. eapply external_call_mem_inject_gen; eauto.
-  apply globals_symbols_inject; auto.
-Qed.
 
 Lemma find_function_inject:
   forall j ros rs fd trs,
@@ -925,6 +882,50 @@ Proof.
   exploit defs_inject; eauto. intros (A & B & C).
   rewrite <- Genv.find_funct_ptr_iff in A. 
   auto.
+Qed.
+
+Lemma stack_equiv_inv_step:
+  forall S1 t S2
+    (STEP: step fn_stack_requirements ge S1 t S2)
+    S1' (MS: match_states S1 S1')
+    S2' (STEP': step fn_stack_requirements tge S1' t S2')
+    (SEI: stack_equiv_inv S1 S1'),
+    stack_equiv_inv S2 S2'.
+Proof.
+  intros.
+  inv STEP; inv MS; inv STEP'; try congruence;
+    unfold stack_equiv_inv in *; simpl in *; repeat rewrite_stack_blocks; eauto using stack_equiv_tail.
+  - rewrite H in H8; inv H8.
+    edestruct find_function_inject as (FFT & KEPT').
+    eapply match_stacks_preserves_globals; eauto.
+    eauto. destr. eapply REGINJ.
+    apply KEPT. red. exists pc. setoid_rewrite H. eexists; split; eauto. simpl. auto.
+    rewrite FFT in H9; inv H9.
+    repeat constructor; auto.
+  - revert SEI. rewrite <- (Mem.alloc_stack_blocks _ _ _ _ _ H).
+    rewrite <- (Mem.alloc_stack_blocks _ _ _ _ _ H7).
+    intro STRUCT.
+    rewrite EQ1, EQ0 in STRUCT. inv STRUCT; constructor; auto.
+    constructor; auto.
+Qed.
+
+Lemma external_call_inject:
+  forall ef vargs m1 t vres m2 f g m1' vargs',
+  meminj_preserves_globals f ->
+  external_call ef ge vargs m1 t vres m2 ->
+  Mem.inject f g m1 m1' ->
+  Val.inject_list f vargs vargs' ->
+  exists f', exists vres', exists m2',
+    external_call ef tge vargs' m1' t vres' m2'
+    /\ Val.inject f' vres vres'
+    /\ Mem.inject f' g m2 m2'
+    /\ Mem.unchanged_on (loc_unmapped f) m1 m2
+    /\ Mem.unchanged_on (loc_out_of_reach f m1) m1' m2'
+    /\ inject_incr f f'
+    /\ inject_separated f f' m1 m1'.
+Proof.
+  intros. eapply external_call_mem_inject_gen; eauto.
+  apply globals_symbols_inject; auto.
 Qed.
 
 Lemma eval_builtin_arg_inject:
@@ -999,18 +1000,23 @@ Proof.
   eapply match_stacks_preserves_globals; eauto. eauto. eauto. intuition.
 Qed.
 
-
+Lemma nextblock_maybe_push:
+  forall (b: bool) m,
+    Mem.nextblock (if b then m else Mem.push_new_stage m) = Mem.nextblock m.
+Proof.
+  intros;   destr; rewrite ?Mem.push_new_stage_nextblock; auto.
+Qed.
 
 Theorem step_simulation:
   forall S1 t S2, step fn_stack_requirements ge S1 t S2 ->
              forall S1' (MS: match_states S1 S1')
-               (SI1: stack_inv S1)
+               (* (SI1: stack_inv S1) *)
                (SI2: stack_inv S1')
                (STRUCT: stack_equiv_inv S1 S1')
              ,
   exists S2', step fn_stack_requirements tge S1' t S2' /\ match_states S2 S2'.
 Proof.
-  induction 1; intros; inv MS; inv SI1; inv SI2; red in STRUCT; simpl in STRUCT.
+  induction 1; intros; inv MS; (* inv SI1; *) inv SI2; red in STRUCT; simpl in STRUCT.
 
 - (* nop *)
   econstructor; split.
@@ -1074,10 +1080,17 @@ Proof.
   econstructor; split. eapply exec_Icall; eauto.
   eapply ros_is_function_translated; eauto.
   econstructor; eauto.
+  rewrite ! Mem.push_new_stage_nextblock.
   econstructor; eauto.
-  change (Mem.valid_block m sp0). eapply Mem.valid_block_inject_1; eauto.
+  change (Mem.valid_block m sp0); eapply Mem.valid_block_inject_1; eauto.
   change (Mem.valid_block tm tsp). eapply Mem.valid_block_inject_2; eauto.
-  apply regs_inject; auto. congruence.
+  apply regs_inject; auto.
+  eapply Mem.mem_inject_ext.
+  apply Mem.push_new_stage_inject. eauto.
+  rewrite_stack_blocks.
+  simpl. intros. unfold flat_frameinj.
+  destr. subst. reflexivity.
+  repeat destr; try omega. simpl. rewrite Nat.succ_pred by omega. auto.
   
 - (* tailcall *)
   exploit find_function_inject.
@@ -1096,14 +1109,6 @@ Proof.
   + eapply Mem.mem_inject_ext. eauto.
     unfold flat_frameinj.
     erewrite <- Mem.free_stack_blocks; eauto.
-  + intros; eapply Mem.noperm_top.
-    repeat rewrite_stack_blocks.
-    inv MSA0.
-    unfold in_frame, get_frame_blocks. rewrite BLOCKS. intros ? [EQ|[]]; subst.
-    intros; intro P. eapply Mem.perm_free_2; eauto.
-    
-    exploit Mem.agree_perms_mem. rewrite <- H7. left; reflexivity. left; reflexivity. rewrite BLOCKS; left; reflexivity.
-    eapply Mem.perm_free_3; eauto. congruence.
   
 - (* builtin *)
   exploit eval_builtin_args_inject; eauto.
@@ -1169,7 +1174,7 @@ Proof.
     intros. destruct (eq_block b1 stk).
     subst b1. rewrite F in H2; inv H2. split; apply Ple_refl.
     rewrite G in H2 by auto. congruence. }
-    exploit Mem.record_push_inject_flat. 8: eauto.
+    exploit Mem.record_push_inject_flat. 8: instantiate (5:= true); simpl; eauto.
     rewrite_stack_blocks. eauto.
     instantiate (1 := make_singleton_frame_adt tstk (fn_stacksize f) sz).
     {
@@ -1202,8 +1207,8 @@ Proof.
       red in JB; xomega.
     }
     reflexivity.
-    intro; subst. specialize (TAILNOPERM eq_refl). inv TAILNOPERM.
-    rewrite_stack_blocks. rewrite <- H1. constructor.
+    intros _.
+    rewrite_stack_blocks. inv TOPNOPERM. constructor.
     red in H2. red.
     intros. intro P.
     eapply Mem.perm_alloc_inv in P; eauto.
@@ -1220,6 +1225,12 @@ Proof.
   exploit external_call_inject; eauto.
   eapply match_stacks_preserves_globals; eauto.
   intros (j' & tres & tm' & A & B & C & D & E & F & G).
+  exploit Mem.unrecord_stack_block_inject_parallel_flat. 2: eauto.
+  rewrite_stack_blocks. eauto.
+  repeat rewrite_stack_blocks.
+  apply Z.eq_le_incl.
+  apply stack_equiv_fsize. apply stack_equiv_tail; auto.
+  intros (m2' & USB & INJ & T).
   econstructor; split.
   eapply exec_function_external; eauto.
   eapply match_states_return with (j := j'); eauto.
@@ -1227,9 +1238,8 @@ Proof.
   apply match_stacks_incr with j; auto.
   intros. exploit G; eauto. intros [P Q].
   unfold Mem.valid_block in *; xomega.
-  eapply external_call_nextblock; eauto.
-  eapply external_call_nextblock; eauto.
-  erewrite <- external_call_stack_blocks; eauto.
+  eapply Ple_trans. eapply external_call_nextblock; eauto. erewrite Mem.unrecord_stack_block_nextblock with (m'0 := m''); eauto. xomega.
+  eapply Ple_trans. eapply external_call_nextblock; eauto. erewrite Mem.unrecord_stack_block_nextblock with (m'0 := m2'); eauto. xomega.
     
 - (* return *)
   inv STACKS. econstructor; split.
@@ -1588,7 +1598,7 @@ Proof.
     eapply Mem.valid_block_inject_2 in FB; eauto. eapply Mem.fresh_block_alloc in FB; eauto. easy.
   - reflexivity.
   - congruence.
-  - exists (Callstate nil f nil m2' (fn_stack_requirements (prog_main tp)) false); split.
+  - exists (Callstate nil f nil (Mem.push_new_stage m2') (fn_stack_requirements (prog_main tp))); split.
     econstructor; eauto.
     + fold tge. erewrite match_prog_main by eauto. auto.
     + destruct TRANSF. rewrite match_prog_main0.
@@ -1614,15 +1624,21 @@ Proof.
               eapply Genv.find_def_not_fresh in H6; eauto.
               eapply Mem.fresh_block_alloc in H6; eauto. easy.
         -- unfold ge. erewrite Genv.init_mem_genv_next by eauto.
+           rewrite Mem.push_new_stage_nextblock.
            rewrite (Mem.record_stack_block_nextblock _ _ _ H5).
            rewrite Mem.push_new_stage_nextblock.
            rewrite (Mem.nextblock_alloc _ _ _ _ _ H4). xomega.
         -- unfold tge. erewrite Genv.init_mem_genv_next by eauto.
+           rewrite Mem.push_new_stage_nextblock.
            rewrite (Mem.record_stack_block_nextblock _ _ _ RSB).
-           rewrite Mem.push_new_stage_nextblock.                      
+           rewrite Mem.push_new_stage_nextblock.
            rewrite (Mem.nextblock_alloc _ _ _ _ _ ALLOC). xomega.
-      * congruence.
-      
+      * eapply Mem.mem_inject_ext.
+        apply Mem.push_new_stage_inject. eauto.
+        rewrite_stack_blocks.
+        simpl. intros. unfold flat_frameinj.
+        destr. subst. reflexivity.
+        repeat destr; try omega. simpl. rewrite Nat.succ_pred by omega. auto.
 Qed.
 
 Lemma stack_equiv_inv_initial:
@@ -1635,16 +1651,9 @@ Proof.
   intros S1 S2 IS1 IS2 MS.
   inv IS1; inv IS2; inv MS.
   red. simpl.
-  edestruct (Mem.record_stack_blocks_stack_eq _ _ _ H4) as (tf & r & EQ1 & EQ2).
-  rewrite EQ2.
-  rewrite Mem.push_new_stage_stack in EQ1; inv EQ1.
-  edestruct (Mem.record_stack_blocks_stack_eq _ _ _ H10) as (ttf & tr & EQ3 & EQ4).
-  rewrite EQ4.
-  rewrite Mem.push_new_stage_stack in EQ3; inv EQ3.
-  constructor; auto.
   repeat rewrite_stack_blocks.
-  erewrite ! Genv.init_mem_stack_adt; eauto. constructor.
   repeat constructor.
+  erewrite ! Genv.init_mem_stack_adt; eauto. constructor.
 Qed.
 
 Lemma transf_final_states:
@@ -1658,20 +1667,20 @@ Lemma transf_program_correct_1:
   forward_simulation (semantics fn_stack_requirements p) (semantics fn_stack_requirements tp).
 Proof.
   intros.
-  eapply forward_simulation_step with (match_states := fun s1 s2 => match_states s1 s2 /\ stack_equiv_inv s1 s2 /\ stack_inv s1 /\ stack_inv s2).
+  eapply forward_simulation_step with (match_states := fun s1 s2 => match_states s1 s2 /\ stack_equiv_inv s1 s2 /\ stack_inv s2).
   - exploit globals_symbols_inject. apply init_meminj_preserves_globals. intros [A B]. exact A.
   - simpl; intros s1 IS. edestruct transf_initial_states as (s2 & IS2 & MS); eauto.
     exploit stack_equiv_inv_initial; eauto. intro SEI.
     eexists; split; eauto. split; auto. split; auto.
-    split; eapply stack_inv_initial; eauto.
+    eapply stack_inv_initial; eauto.
   - intros s1 s2 r (MS & _) FS.
     eapply transf_final_states; eauto.
-  - simpl. intros s1 t s1' STEP s2 (MS & SEI & SI1 & SI2).
+  - simpl. intros s1 t s1' STEP s2 (MS & SEI & SI2).
     edestruct step_simulation as (s2' & STEP' & MS'); eauto.
     eexists; split; eauto.
     split. auto.
     split. eapply stack_equiv_inv_step; eauto.
-    split; eapply stack_inv_inv; eauto.
+    eapply stack_inv_inv; eauto.
 Qed.
 
 End SOUNDNESS.
